src/Semantics/Stack.thy
@@ -16,7 +16,7 @@ begin
     by allocating a new block of memory for each variable.\<close>
   definition alloc_vdecls :: "vdecl list \<Rightarrow> memory \<hookrightarrow> (valuation\<times>memory)" where
     "alloc_vdecls l \<mu> \<equiv> efold (\<lambda>(vname,ty) (vals,\<mu>). do {
-      (addr,\<mu>) \<leftarrow> alloc ty \<mu>;
+      (addr,\<mu>) \<leftarrow> alloc ty True \<mu>;
       let vals = vals(vname \<mapsto> addr);
       return (vals,\<mu>)
       }) l (Map.empty,\<mu>)"
@@ -26,7 +26,7 @@ begin
     "alloc_params vdecls vs \<mu> \<equiv> do {
       assert (length vdecls = length vs) structural_error;
       efold (\<lambda>((name,ty),v) (vals,\<mu>). do {
-        (addr,\<mu>) \<leftarrow> cp_alloc ty v \<mu>;
+        (addr,\<mu>) \<leftarrow> cp_alloc ty True v \<mu>;
         let vals = vals(name \<mapsto> addr);
         return (vals,\<mu>)
       }) (zip vdecls vs) (Map.empty,\<mu>)
@@ -46,28 +46,10 @@ begin
       let names = map fst (fun_decl.params fd @ fun_decl.locals fd);
       efold (\<lambda>x \<mu>. do {
         let addr = the (lv x);
-        free addr \<mu>
+        free True addr \<mu>
       }) names \<mu>
     }"
 
-  (* TODO/FIXME/BUG: We should protect memory allocated by stack-frames from being freed explicitely! 
-    In particular for globals, this is important: Currently, our semantics allows
-      "free &x" where x is a global!
-
-    While we can argue that this will yield an error late for locals, i.e., on returning 
-    from the function, it still seems somewhat scary to allow such a behaviour.
-
-    Ideas for solution:
-      1) Allocate frame with an T[1] - indirection, such that you never obtain a block pointer
-          by referencing locals, globals, or parameters.
-
-      2) Flag blocks as being statically allocated. Check for that on explicit free instruction.
-
-      #2 seems somewhat cleaner by explicitly addressing the problem, while #1 is a hack 
-        indirectly exploiting that only block-base pointers can be freed, assuming that one
-        can never obtain the base-pointer from a deeper pointer.
-
-    *)  
 
   type_synonym state = "stack \<times> valuation \<times> memory"  
 
